theories/machine_parameters.v
@@ -38,3 +38,21 @@ Definition encodeInstrW `{MachineParameters} : instr → Word :=
 Lemma decode_encode_instrW_inv `{MachineParameters} (i: instr):
   decodeInstrW (encodeInstrW i) = i.
 Proof. apply decode_encode_instr_inv. Qed.
+
+Global Instance decode_encode_cancel `{MachineParameters}: Cancel (=) decodeInstr encodeInstr.
+Proof. intro. eapply decode_encode_instr_inv. Qed.
+
+Global Instance decode_encode_cancelW `{MachineParameters}: Cancel (=) decodeInstrW encodeInstrW.
+Proof. intro. eapply decode_encode_instrW_inv. Qed.
+
+Global Instance decode_instr_surj `{MachineParameters}: Surj (=) decodeInstr.
+Proof. eapply cancel_surj. Qed.
+
+Global Instance encode_instr_inj `{MachineParameters}: Inj (=) (=) encodeInstr.
+Proof. eapply cancel_inj. Qed.
+
+Global Instance decode_instrW_surj `{MachineParameters}: Surj (=) decodeInstrW.
+Proof. eapply cancel_surj. Qed.
+
+Global Instance encode_instrw_inj `{MachineParameters}: Inj (=) (=) encodeInstrW.
+Proof. eapply cancel_inj. Qed.
